Weidenbach_Book/IsaSAT/IsaSAT_LLVM.thy
@@ -427,6 +427,8 @@ begin
     IsaSAT_Profile_REDUCE is \<open>PROFILE_CST IsaSAT_Profile_REDUCE\<close>
     IsaSAT_Profile_GC is \<open>PROFILE_CST IsaSAT_Profile_GC\<close>
     IsaSAT_Profile_ANALYZE is \<open>PROFILE_CST IsaSAT_Profile_ANALYZE\<close>
+    IsaSAT_Profile_MINIMIZATION is \<open>PROFILE_CST IsaSAT_Profile_MINIMIZATION\<close>
+    IsaSAT_Profile_INITIALISATION is \<open>PROFILE_CST IsaSAT_Profile_INITIALISATION\<close>
   defines \<open>
      typedef int8_t CBOOL;
      typedef int8_t PROFILE_CST;
