Weidenbach_Book/IsaSAT/IsaSAT_Profile_LLVM.thy
@@ -8,6 +8,8 @@ sepref_register IsaSAT_Profile.start
   IsaSAT_Profile.ANALYZE
   IsaSAT_Profile.GC
   IsaSAT_Profile.REDUCE
+  IsaSAT_Profile.INITIALISATION
+  IsaSAT_Profile.MINIMIZATION
 
 sepref_def start_profile
   is \<open>RETURN o IsaSAT_Profile.start\<close>
@@ -47,6 +49,18 @@ sepref_def IsaSAT_Profile_REDUCE
   by sepref
 
 
+sepref_def IsaSAT_Profile_MINIMIZATION
+  is \<open>uncurry0 (RETURN IsaSAT_Profile.MINIMIZATION)\<close>
+  :: \<open>unit_assn\<^sup>k \<rightarrow>\<^sub>a word_assn\<close>
+  unfolding IsaSAT_Profile.MINIMIZATION_def
+  by sepref
+
+sepref_def IsaSAT_Profile_INITIALISATION
+  is \<open>uncurry0 (RETURN IsaSAT_Profile.INITIALISATION)\<close>
+  :: \<open>unit_assn\<^sup>k \<rightarrow>\<^sub>a word_assn\<close>
+  unfolding IsaSAT_Profile.INITIALISATION_def
+  by sepref
+
 experiment begin
 
 export_llvm
@@ -54,6 +68,8 @@ export_llvm
     IsaSAT_Profile_REDUCE is \<open>PROFILE_CST IsaSAT_Profile_REDUCE\<close>
     IsaSAT_Profile_GC is \<open>PROFILE_CST IsaSAT_Profile_GC\<close>
     IsaSAT_Profile_ANALYZE is \<open>PROFILE_CST IsaSAT_Profile_ANALYZE\<close>
+    IsaSAT_Profile_MINIMIZATION is \<open>PROFILE_CST IsaSAT_Profile_MINIMIZATION\<close>
+    IsaSAT_Profile_INITIALISATION is \<open>PROFILE_CST IsaSAT_Profile_INITIALISATION\<close>
     defines \<open>
        typedef int8_t PROFILE_CST;
   \<close>
